Add support for reifying `zrange` and `option`
This is needed to reify statements for the rewriter.

src/Language.v
@@ -15,7 +15,7 @@ Require Import Crypto.Util.CPSNotations.
 Require Import Crypto.Util.Notations.
 Require Import Crypto.Util.Tactics.RunTacticAsConstr.
 Require Import Crypto.Util.Tactics.DebugPrint.
-Import ListNotations. Local Open Scope bool_scope. Local Open Scope Z_scope.
+Import Coq.Lists.List ListNotations. Local Open Scope bool_scope. Local Open Scope Z_scope.
 
 Module Compilers.
   Local Set Boolean Equality Schemes.
@@ -293,8 +293,8 @@ Module Compilers.
   Module base.
     Local Notation einterp := type.interp.
     Module type.
-      Inductive base := unit | Z | bool | nat. (* Not Variant because COQBUG(https://github.com/coq/coq/issues/7738) *)
-      Inductive type := type_base (t : base) | prod (A B : type) | list (A : type).
+      Inductive base := unit | Z | bool | nat | zrange. (* Not Variant because COQBUG(https://github.com/coq/coq/issues/7738) *)
+      Inductive type := type_base (t : base) | prod (A B : type) | list (A : type) | option (A : type).
       Global Coercion type_base : base >-> type.
     End type.
     Global Coercion type.type_base : type.base >-> type.type.
@@ -305,12 +305,14 @@ Module Compilers.
          | type.Z => BinInt.Z
          | type.bool => Datatypes.bool
          | type.nat => Datatypes.nat
+         | type.zrange => zrange
          end.
     Fixpoint interp (ty : type)
       := match ty with
          | type.type_base t => base_interp t
          | type.prod A B => interp A * interp B
          | type.list A => Datatypes.list (interp A)
+         | type.option A => Datatypes.option (interp A)
          end%type.
 
     Definition try_make_base_transport_cps
@@ -321,11 +323,13 @@ Module Compilers.
          | type.Z, type.Z
          | type.bool, type.bool
          | type.nat, type.nat
+         | type.zrange, type.zrange
            => (return (Some id))
          | type.unit, _
          | type.Z, _
          | type.bool, _
          | type.nat, _
+         | type.zrange, _
            => (return None)
          end%cps.
     Fixpoint try_make_transport_cps
@@ -339,9 +343,11 @@ Module Compilers.
                 trB <-- try_make_transport_cps (fun B => P (type.prod _ B)) _ _;
               return (Some (fun v => trB (trA v))))
          | type.list A, type.list A' => try_make_transport_cps (fun A => P (type.list A)) A A'
+         | type.option A, type.option A' => try_make_transport_cps (fun A => P (type.option A)) A A'
          | type.type_base _, _
          | type.prod _ _, _
          | type.list _, _
+         | type.option _, _
            => (return None)
          end%cps.
 
@@ -351,31 +357,6 @@ Module Compilers.
 
     Definition try_transport (P : type -> Type) (t1 t2 : type) (v : P t1) : option (P t2)
       := try_transport_cps P t1 t2 v _ id.
-    (*
-    Fixpoint try_transport
-             (P : type -> Type) (t1 t2 : type) : P t1 -> option (P t2)
-      := match t1, t2 return P t1 -> option (P t2) with
-         | type.unit, type.unit
-         | type.Z, type.Z
-         | type.bool, type.bool
-         | type.nat, type.nat
-           => @Some _
-         | type.list A, type.list A'
-           => @try_transport (fun A => P (type.list A)) A A'
-         | type.prod s d, type.prod s' d'
-           => fun v
-              => (v <- (try_transport (fun s => P (type.prod s d)) s s' v);
-                    (try_transport (fun d => P (type.prod s' d)) d d' v))%option
-
-         | type.unit, _
-         | type.Z, _
-         | type.bool, _
-         | type.nat, _
-         | type.prod _ _, _
-         | type.list _, _
-           => fun _ => None
-         end.
-     *)
 
     Ltac reify_base ty :=
       let __ := Reify.debug_enter_reify_base_type ty in
@@ -384,6 +365,7 @@ Module Compilers.
       | Datatypes.nat => type.nat
       | Datatypes.bool => type.bool
       | BinInt.Z => type.Z
+      | zrange => type.zrange
       | interp (type.type_base ?T) => T
       | @einterp type interp (@Compilers.type.base type (type.type_base ?T)) => T
       | _ => let __ := match goal with
@@ -401,6 +383,9 @@ Module Compilers.
       | Datatypes.list ?T
         => let rT := reify T in
           constr:(type.list rT)
+      | Datatypes.option ?T
+        => let rT := reify T in
+          constr:(type.option rT)
       | interp ?T => T
       | @einterp type interp (@Compilers.type.base type ?T) => T
       | ?ty => let rT := reify_base ty in
@@ -616,6 +601,9 @@ Module Compilers.
         | match ?x with Datatypes.pair a b => @?f a b end
           => let T := type of term in
              reify_rec (@prod_rect _ _ (fun _ => T) f x)
+        | match ?x with ZRange.Build_zrange a b => @?f a b end
+          => let T := type of term in
+             reify_rec (@ZRange.zrange_rect (fun _ => T) f x)
         | match ?x with nil => ?N | cons a b => @?C a b end
           => let T := type of term in
              reify_rec (@list_case _ (fun _ => T) N C x)
@@ -892,13 +880,17 @@ Module Compilers.
         | Z_log2_up : ident (Z -> Z)
         | Z_eqb : ident (Z -> Z -> bool)
         | Z_leb : ident (Z -> Z -> bool)
+        | Z_ltb : ident (Z -> Z -> bool)
         | Z_geb : ident (Z -> Z -> bool)
+        | Z_gtb : ident (Z -> Z -> bool)
         | Z_of_nat : ident (nat -> Z)
         | Z_to_nat : ident (Z -> nat)
         | Z_shiftr : ident (Z -> Z -> Z)
         | Z_shiftl : ident (Z -> Z -> Z)
         | Z_land : ident (Z -> Z -> Z)
         | Z_lor : ident (Z -> Z -> Z)
+        | Z_min : ident (Z -> Z -> Z)
+        | Z_max : ident (Z -> Z -> Z)
         | Z_bneg : ident (Z -> Z)
         | Z_lnot_modulo : ident (Z -> Z -> Z)
         | Z_mul_split : ident (Z -> Z -> Z -> Z * Z)
@@ -911,8 +903,13 @@ Module Compilers.
         | Z_add_modulo : ident (Z -> Z -> Z -> Z)
         | Z_rshi : ident (Z -> Z -> Z -> Z -> Z)
         | Z_cc_m : ident (Z -> Z -> Z)
-        | Z_cast (range : zrange) : ident (Z -> Z)
-        | Z_cast2 (range : zrange * zrange) : ident ((Z * Z) -> (Z * Z))
+        | Z_cast (range : ZRange.zrange) : ident (Z -> Z)
+        | Z_cast2 (range : ZRange.zrange * ZRange.zrange) : ident ((Z * Z) -> (Z * Z))
+        | option_Some {A:base.type} : ident (A -> option A)
+        | option_None {A:base.type} : ident (option A)
+        | option_rect {A P : base.type} : ident ((A -> P) -> (unit -> P) -> option A -> P)
+        | Build_zrange : ident (Z -> Z -> zrange)
+        | zrange_rect {P:base.type} : ident ((Z -> Z -> P) -> zrange -> P)
         | fancy_add (log2wordmax : BinInt.Z) (imm : BinInt.Z) : ident (Z * Z -> Z * Z)
         | fancy_addc (log2wordmax : BinInt.Z) (imm : BinInt.Z) : ident (Z * Z * Z -> Z * Z)
         | fancy_sub (log2wordmax : BinInt.Z) (imm : BinInt.Z) : ident (Z * Z -> Z * Z)
@@ -927,30 +924,34 @@ Module Compilers.
         | fancy_sell : ident (Z * Z * Z -> Z)
         | fancy_addm : ident (Z * Z * Z -> Z)
         .
+        Notation Some := option_Some.
+        Notation None := option_None.
 
         Global Arguments Z_cast2 _%zrange_scope.
 
-        Definition to_fancy {s d : base.type} (idc : ident (s -> d)) : option (fancy.ident s d)
-          := match idc in ident t return option match t with
+        Definition to_fancy {s d : base.type} (idc : ident (s -> d)) : Datatypes.option (fancy.ident s d)
+          := match idc in ident t return Datatypes.option match t with
                                                 | type.base s -> type.base d => fancy.ident s d
                                                 | _ => Datatypes.unit
                                                 end%etype with
-             | fancy_add log2wordmax imm => Some (fancy.with_wordmax log2wordmax (fancy.add imm))
-             | fancy_addc log2wordmax imm => Some (fancy.with_wordmax log2wordmax (fancy.addc imm))
-             | fancy_sub log2wordmax imm => Some (fancy.with_wordmax log2wordmax (fancy.sub imm))
-             | fancy_subb log2wordmax imm => Some (fancy.with_wordmax log2wordmax (fancy.subb imm))
-             | fancy_mulll log2wordmax => Some (fancy.with_wordmax log2wordmax fancy.mulll)
-             | fancy_mullh log2wordmax => Some (fancy.with_wordmax log2wordmax fancy.mullh)
-             | fancy_mulhl log2wordmax => Some (fancy.with_wordmax log2wordmax fancy.mulhl)
-             | fancy_mulhh log2wordmax => Some (fancy.with_wordmax log2wordmax fancy.mulhh)
-             | fancy_rshi log2wordmax x => Some (fancy.with_wordmax log2wordmax (fancy.rshi x))
-             | fancy_selc => Some fancy.selc
-             | fancy_selm log2wordmax => Some (fancy.with_wordmax log2wordmax fancy.selm)
-             | fancy_sell => Some fancy.sell
-             | fancy_addm => Some fancy.addm
-             | _ => None
+             | fancy_add log2wordmax imm => Datatypes.Some (fancy.with_wordmax log2wordmax (fancy.add imm))
+             | fancy_addc log2wordmax imm => Datatypes.Some (fancy.with_wordmax log2wordmax (fancy.addc imm))
+             | fancy_sub log2wordmax imm => Datatypes.Some (fancy.with_wordmax log2wordmax (fancy.sub imm))
+             | fancy_subb log2wordmax imm => Datatypes.Some (fancy.with_wordmax log2wordmax (fancy.subb imm))
+             | fancy_mulll log2wordmax => Datatypes.Some (fancy.with_wordmax log2wordmax fancy.mulll)
+             | fancy_mullh log2wordmax => Datatypes.Some (fancy.with_wordmax log2wordmax fancy.mullh)
+             | fancy_mulhl log2wordmax => Datatypes.Some (fancy.with_wordmax log2wordmax fancy.mulhl)
+             | fancy_mulhh log2wordmax => Datatypes.Some (fancy.with_wordmax log2wordmax fancy.mulhh)
+             | fancy_rshi log2wordmax x => Datatypes.Some (fancy.with_wordmax log2wordmax (fancy.rshi x))
+             | fancy_selc => Datatypes.Some fancy.selc
+             | fancy_selm log2wordmax => Datatypes.Some (fancy.with_wordmax log2wordmax fancy.selm)
+             | fancy_sell => Datatypes.Some fancy.sell
+             | fancy_addm => Datatypes.Some fancy.addm
+             | _ => Datatypes.None
              end.
       End with_scope.
+      Notation Some := option_Some.
+      Notation None := option_None.
 
       Section gen.
         Context (cast_outside_of_range : zrange -> BinInt.Z -> BinInt.Z).
@@ -1036,7 +1037,9 @@ Module Compilers.
              | Z_modulo => Z.modulo
              | Z_eqb => Z.eqb
              | Z_leb => Z.leb
+             | Z_ltb => Z.ltb
              | Z_geb => Z.geb
+             | Z_gtb => Z.gtb
              | Z_log2 => Z.log2
              | Z_log2_up => Z.log2_up
              | Z_of_nat => Z.of_nat
@@ -1045,6 +1048,8 @@ Module Compilers.
              | Z_shiftl => Z.shiftl
              | Z_land => Z.land
              | Z_lor => Z.lor
+             | Z_min => Z.min
+             | Z_max => Z.max
              | Z_mul_split => Z.mul_split
              | Z_add_get_carry => Z.add_get_carry_full
              | Z_add_with_carry => Z.add_with_carry
@@ -1059,6 +1064,12 @@ Module Compilers.
              | Z_cc_m => Z.cc_m
              | Z_cast r => cast r
              | Z_cast2 (r1, r2) => fun '(x1, x2) => (cast r1 x1, cast r2 x2)
+             | Some A => @Datatypes.Some _
+             | None A => @Datatypes.None _
+             | option_rect A P
+               => fun S_case N_case o => @Datatypes.option_rect _ _ S_case (N_case tt) o
+             | Build_zrange => ZRange.Build_zrange
+             | zrange_rect A => @ZRange.zrange_rect _
              | fancy_add _ _ as idc
              | fancy_addc _ _ as idc
              | fancy_sub _ _ as idc
@@ -1079,6 +1090,8 @@ Module Compilers.
       Definition cast_outside_of_range (r : zrange) (v : BinInt.Z) : BinInt.Z.
       Proof. exact v. Qed.
     End with_base.
+    Notation Some := option_Some.
+    Notation None := option_None.
 
     (** Interpret identifiers where [Z_cast] is an opaque identity
         function when the value is not inside the range *)
@@ -1087,6 +1100,7 @@ Module Compilers.
     Notation LiteralZ := (@Literal base.type.Z).
     Notation LiteralBool := (@Literal base.type.bool).
     Notation LiteralNat := (@Literal base.type.nat).
+    Notation LiteralZRange := (@Literal base.type.zrange).
 
     (** TODO: MOVE ME? *)
     Module Thunked.
@@ -1098,6 +1112,8 @@ Module Compilers.
         := ListUtil.list_case (fun _ => P) (N tt) C ls.
       Definition nat_rect P (O_case : unit -> P) (S_case : nat -> P -> P) (n : nat) : P
         := Datatypes.nat_rect (fun _ => P) (O_case tt) S_case n.
+      Definition option_rect {A} P (S_case : A -> P) (N_case : unit -> P) (o : option A) : P
+        := Datatypes.option_rect (fun _ => P) S_case (N_case tt) o.
     End Thunked.
 
     Ltac require_primitive_const term :=
@@ -1113,6 +1129,10 @@ Module Compilers.
       | xI ?p => require_primitive_const p
       | xO ?p => require_primitive_const p
       | xH => idtac
+      | Datatypes.Some ?x => require_primitive_const x
+      | Datatypes.None => idtac
+      | ZRange.Build_zrange ?x ?y
+        => require_primitive_const x; require_primitive_const y
       | ?term => fail 0 "Not a known const:" term
       end.
     Ltac is_primitive_const term :=
@@ -1175,6 +1195,16 @@ Module Compilers.
         | @Thunked.bool_rect ?T
           => let rT := base.reify T in
              then_tac (@ident.bool_rect rT)
+        | @Datatypes.option_rect ?A ?T0 ?PSome ?PNone
+          => lazymatch (eval cbv beta in T0) with
+             | fun _ => ?T => reify_rec (@Thunked.option_rect A T PSome (fun _ : Datatypes.unit => PNone))
+             | T0 => else_tac ()
+             | ?T' => reify_rec (@Datatypes.option_rect A T' PSome PNone)
+             end
+        | @Thunked.option_rect ?A ?T
+          => let rA := base.reify A in
+             let rT := base.reify T in
+             then_tac (@ident.option_rect rA rT)
         | @Datatypes.prod_rect ?A ?B ?T0
           => lazymatch (eval cbv beta in T0) with
             | fun _ => ?T
@@ -1185,6 +1215,14 @@ Module Compilers.
             | T0 => else_tac ()
             | ?T' => reify_rec (@Datatypes.prod_rect A B T')
             end
+        | @ZRange.zrange_rect ?T0
+          => lazymatch (eval cbv beta in T0) with
+             | fun _ => ?T
+               => let rT := base.reify T in
+                  then_tac (@ident.zrange_rect rT)
+             | T0 => else_tac ()
+             | ?T' => reify_rec (@ZRange.zrange_rect T')
+             end
         | @Datatypes.nat_rect ?T0 ?P0
           => lazymatch (eval cbv beta in T0) with
              | fun _ => _ -> _ => else_tac ()
@@ -1277,13 +1315,17 @@ Module Compilers.
         | Z.modulo => then_tac ident.Z_modulo
         | Z.eqb => then_tac ident.Z_eqb
         | Z.leb => then_tac ident.Z_leb
+        | Z.ltb => then_tac ident.Z_ltb
         | Z.geb => then_tac ident.Z_geb
+        | Z.gtb => then_tac ident.Z_gtb
         | Z.log2 => then_tac ident.Z_log2
         | Z.log2_up => then_tac ident.Z_log2_up
         | Z.shiftl => then_tac ident.Z_shiftl
         | Z.shiftr => then_tac ident.Z_shiftr
         | Z.land => then_tac ident.Z_land
         | Z.lor => then_tac ident.Z_lor
+        | Z.min => then_tac ident.Z_min
+        | Z.max => then_tac ident.Z_max
         | Z.bneg => then_tac ident.Z_bneg
         | Z.lnot_modulo => then_tac ident.Z_lnot_modulo
         | Z.of_nat => then_tac ident.Z_of_nat
@@ -1298,6 +1340,14 @@ Module Compilers.
         | Z.add_modulo => then_tac ident.Z_add_modulo
         | Z.rshi => then_tac ident.Z_rshi
         | Z.cc_m => then_tac ident.Z_cc_m
+        | ident.cast _ => then_tac ident.Z_cast
+        | @Some ?A
+          => let rA := base.reify A in
+             then_tac (@ident.Some rA)
+        | @None ?A
+          => let rA := base.reify A in
+             then_tac (@ident.None rA)
+        | ZRange.Build_zrange => then_tac ident.Build_zrange
         | _ => else_tac ()
         end
       end.
@@ -1309,6 +1359,13 @@ Module Compilers.
            (fun x _ xs => expr.Ident ident.cons @ x @ xs)%expr
            ls.
 
+    Definition reify_option {var} {t} (v : option (@expr.expr base.type ident var (type.base t))) : @expr.expr base.type ident var (type.base (base.type.option t))
+      := Datatypes.option_rect
+           (fun _ => _)
+           (fun x => expr.Ident ident.Some @ x)%expr
+           (expr.Ident ident.None)
+           v.
+
     Fixpoint smart_Literal {var} {t:base.type} : base.interp t -> @expr.expr base.type ident var (type.base t)
       := match t with
          | base.type.type_base t => fun v => expr.Ident (ident.Literal v)
@@ -1318,6 +1375,9 @@ Module Compilers.
          | base.type.list A
            => fun v : list (base.interp A)
               => reify_list (List.map (@smart_Literal var A) v)
+         | base.type.option A
+           => fun v : option (base.interp A)
+              => reify_option (option_map (@smart_Literal var A) v)
          end%expr.
 
     Module Export Notations.
@@ -1354,7 +1414,7 @@ Module Compilers.
       Notation "x 'mod' y" := (#Z_modulo @ x @ y)%expr : expr_scope.
       Notation "- x" := (#Z_opp @ x)%expr : expr_scope.
       Global Arguments gen_interp _ _ !_.
-
+      Global Arguments ident.Z_cast _%zrange_scope.
       Global Arguments ident.Z_cast2 _%zrange_scope.
     End Notations.
   End ident.
@@ -1519,6 +1579,42 @@ Module Compilers.
            | Some (ident.nil _) => true
            | _ => false
            end.
+      Definition invert_None {t} (e : expr (base.type.option t)) : bool
+        := match invert_Ident e with
+           | Some (ident.None _) => true
+           | _ => false
+           end.
+      Local Notation if_arrow f t
+        := (match t return Type with
+            | (a -> b)%etype => f a b
+            | _ => unit
+            end) (only parsing).
+      Definition invert_Some {t} (e : expr (base.type.option t))
+        : option (expr t)
+        := match invert_AppIdent e with
+           | Some (existT s (idc, e))
+             => match idc in ident.ident t
+                      return if_arrow (fun a b => expr a) t
+                             -> option match t return Type with
+                                       | (a -> type.base (base.type.option t))
+                                         => expr t
+                                       | _ => unit
+                                       end%etype
+                with
+                | ident.Some _ => fun x => Some x
+                | _ => fun _ => None
+                end e
+           | None => None
+           end.
+
+      Definition reflect_option {t} (e : expr (base.type.option t))
+        : option (option (expr t))
+        := match invert_None e, invert_Some e with
+           | true, _ => Some None
+           | _, Some x => Some (Some x)
+           | false, None => None
+           end.
+
       Local Notation if_arrow2 f t
         := (match t return Type with
             | (a -> b -> c)%etype => f a b c
@@ -1590,9 +1686,11 @@ Module Compilers.
              | base.type.Z => (-1)%Z
              | base.type.nat => 0%nat
              | base.type.bool => true
+             | base.type.zrange => r[0~>0]%zrange
              | base.type.list _ => nil
              | base.type.prod A B
                => (@default A, @default B)
+             | base.type.option A => None
              end.
       End base.
       Fixpoint default {t} : type.interp base.interp t
@@ -1611,10 +1709,12 @@ Module Compilers.
                | base.type.prod A B
                  => (@default A, @default B)
                | base.type.list A => #ident.nil
+               | base.type.option A => #ident.None
                | base.type.unit as t
                | base.type.Z as t
                | base.type.nat as t
                | base.type.bool as t
+               | base.type.zrange as t
                  => ##(@type.base.default t)
                end%expr.
         End with_var.
@@ -1649,6 +1749,7 @@ Module Compilers.
   End defaults.
 
   Notation reify_list := ident.reify_list.
+  Notation reify_option := ident.reify_option.
 
   Module GallinaReify.
     Module base.
@@ -1663,10 +1764,14 @@ Module Compilers.
              | base.type.list A as t
                => fun x : list (base.interp A)
                   => reify_list (List.map (@reify A) x)
+             | base.type.option A as t
+               => fun x : option (base.interp A)
+                  => reify_option (option_map (@reify A) x)
              | base.type.unit as t
              | base.type.Z as t
              | base.type.bool as t
              | base.type.nat as t
+             | base.type.zrange as t
                => fun x : base.interp t
                   => (##x)%expr
              end.
