src/AbstractInterpretationWf.v
@@ -305,6 +305,7 @@ Module Compilers.
                 (bottom' : forall A, abstract_domain' A)
                 (abstract_interp_ident : forall t, ident t -> type.interp abstract_domain' t)
                 (extract_list_state : forall A, abstract_domain' (base.type.list A) -> option (list (abstract_domain' A)))
+                (extract_option_state : forall A, abstract_domain' (base.type.option A) -> option (option (abstract_domain' A)))
                 (is_annotated_for : forall t t', ident t -> abstract_domain' t' -> bool).
         Context (abstract_domain'_R : forall t, abstract_domain' t -> abstract_domain' t -> Prop).
         Local Notation abstract_domain_R := (@abstract_domain_R base.type abstract_domain' abstract_domain'_R).
@@ -313,7 +314,8 @@ Module Compilers.
                 {bottom'_Proper : forall t, Proper (abstract_domain'_R t) (bottom' t)}
                 {is_annotated_for_Proper : forall t t', Proper (eq ==> abstract_domain'_R _ ==> eq) (@is_annotated_for t t')}
                 (extract_list_state_length : forall t v1 v2, abstract_domain'_R _ v1 v2 -> option_map (@length _) (extract_list_state t v1) = option_map (@length _) (extract_list_state t v2))
-                (extract_list_state_rel : forall t v1 v2, abstract_domain'_R _ v1 v2 -> forall l1 l2, extract_list_state t v1 = Some l1 -> extract_list_state t v2 = Some l2 -> forall vv1 vv2, List.In (vv1, vv2) (List.combine l1 l2) -> @abstract_domain'_R t vv1 vv2).
+                (extract_list_state_rel : forall t v1 v2, abstract_domain'_R _ v1 v2 -> forall l1 l2, extract_list_state t v1 = Some l1 -> extract_list_state t v2 = Some l2 -> forall vv1 vv2, List.In (vv1, vv2) (List.combine l1 l2) -> @abstract_domain'_R t vv1 vv2)
+                (extract_option_state_rel : forall t v1 v2, abstract_domain'_R _ v1 v2 -> option_eq (option_eq (abstract_domain'_R _)) (extract_option_state t v1) (extract_option_state t v2)).
 
         Local Instance abstract_interp_ident_Proper_arrow s d
           : Proper (eq ==> abstract_domain'_R s ==> abstract_domain'_R d) (abstract_interp_ident (type.arrow s d))
@@ -324,14 +326,14 @@ Module Compilers.
 
           Local Notation update_annotation1 := (@ident.update_annotation var1 abstract_domain' annotate_ident is_annotated_for).
           Local Notation update_annotation2 := (@ident.update_annotation var2 abstract_domain' annotate_ident is_annotated_for).
-          Local Notation annotate1 := (@ident.annotate var1 abstract_domain' annotate_ident abstract_interp_ident extract_list_state is_annotated_for).
-          Local Notation annotate2 := (@ident.annotate var2 abstract_domain' annotate_ident abstract_interp_ident extract_list_state is_annotated_for).
+          Local Notation annotate1 := (@ident.annotate var1 abstract_domain' annotate_ident abstract_interp_ident extract_list_state extract_option_state is_annotated_for).
+          Local Notation annotate2 := (@ident.annotate var2 abstract_domain' annotate_ident abstract_interp_ident extract_list_state extract_option_state is_annotated_for).
           Local Notation annotate_base1 := (@ident.annotate_base var1 abstract_domain' annotate_ident is_annotated_for).
           Local Notation annotate_base2 := (@ident.annotate_base var2 abstract_domain' annotate_ident is_annotated_for).
           Local Notation annotate_with_ident1 := (@ident.annotate_with_ident var1 abstract_domain' annotate_ident is_annotated_for).
           Local Notation annotate_with_ident2 := (@ident.annotate_with_ident var2 abstract_domain' annotate_ident is_annotated_for).
-          Local Notation interp_ident1 := (@ident.interp_ident var1 abstract_domain' annotate_ident bottom' abstract_interp_ident extract_list_state is_annotated_for).
-          Local Notation interp_ident2 := (@ident.interp_ident var2 abstract_domain' annotate_ident bottom' abstract_interp_ident extract_list_state is_annotated_for).
+          Local Notation interp_ident1 := (@ident.interp_ident var1 abstract_domain' annotate_ident bottom' abstract_interp_ident extract_list_state extract_option_state is_annotated_for).
+          Local Notation interp_ident2 := (@ident.interp_ident var2 abstract_domain' annotate_ident bottom' abstract_interp_ident extract_list_state extract_option_state is_annotated_for).
           Local Notation reflect1 := (@reflect base.type ident var1 abstract_domain' annotate1 bottom').
           Local Notation reflect2 := (@reflect base.type ident var2 abstract_domain' annotate2 bottom').
 
@@ -408,7 +410,7 @@ Module Compilers.
                 v1 v2 (Hv : abstract_domain'_R t v1 v2)
                 e1 e2 (He : expr.wf G e1 e2)
             : UnderLets.wf (fun G' => expr.wf G') G (@annotate1 is_let_bound t v1 e1) (@annotate2 is_let_bound t v2 e2).
-          Proof using abstract_interp_ident_Proper annotate_ident_Proper extract_list_state_length extract_list_state_rel is_annotated_for_Proper.
+          Proof using abstract_interp_ident_Proper annotate_ident_Proper extract_list_state_length extract_list_state_rel extract_option_state_rel is_annotated_for_Proper.
             revert dependent G; induction t; intros;
               cbn [ident.annotate]; try apply wf_annotate_base; trivial.
             all: repeat first [ lazymatch goal with
@@ -430,6 +432,13 @@ Module Compilers.
                                      pose proof (extract_list_state_length _ v1 v2 Hv) as Hl;
                                      pose proof (extract_list_state_rel _ v1 v2 Hv) as Hl';
                                      rewrite H, H' in Hl, Hl'; cbv [option_eq option_map] in Hl, Hl'; clear H H'
+                                | [ H : abstract_domain'_R _ ?v1 ?v2, H1 : extract_option_state _ ?v1 = _, H2 : extract_option_state _ ?v2 = _ |- _ ]
+                                  => let H' := fresh in
+                                     pose proof H as H';
+                                     apply extract_option_state_rel in H';
+                                     rewrite H1, H2 in H';
+                                     cbv [option_eq] in H';
+                                     clear H1 H2
                                 | [ H : ?x = ?x |- _ ] => clear H
                                 | [ H : length ?l1 = length ?l2, H' : context[length ?l1] |- _ ] => rewrite H in H'
                                 end
@@ -476,6 +485,9 @@ Module Compilers.
                               | progress rewrite_type_transport_correct
                               | apply conj
                               | congruence
+                              | progress destruct_head' option
+                              | progress cbn [Option.combine option_map UnderLets.splice_option reify_option option_rect] in *
+                              | progress cbn [type.decode f_equal eq_rect fst snd] in *
                               | solve [ wf_t ] ].
           Qed.
 
@@ -492,7 +504,7 @@ Module Compilers.
             end.
           Lemma wf_interp_ident_nth_default (annotate_with_state : bool) G T
             : wf_value_with_lets G (@interp_ident1 annotate_with_state _ (@ident.List_nth_default T)) (@interp_ident2 annotate_with_state _ (@ident.List_nth_default T)).
-          Proof using abstract_interp_ident_Proper annotate_ident_Proper extract_list_state_length extract_list_state_rel is_annotated_for_Proper.
+          Proof using abstract_interp_ident_Proper annotate_ident_Proper extract_list_state_length extract_list_state_rel extract_option_state_rel is_annotated_for_Proper.
             cbv [wf_value_with_lets wf_value ident.interp_ident]; constructor; cbn -[abstract_domain_R abstract_domain].
             { intros; subst.
               destruct_head'_prod; destruct_head'_and; cbn [fst snd] in *.
@@ -600,7 +612,7 @@ Module Compilers.
 
           Lemma wf_interp_ident_not_nth_default (annotate_with_state : bool) G {t} (idc : ident t)
             : wf_value_with_lets G (Base (reflect1 annotate_with_state (###idc)%expr (abstract_interp_ident _ idc))) (Base (reflect2 annotate_with_state (###idc)%expr (abstract_interp_ident _ idc))).
-          Proof using abstract_interp_ident_Proper annotate_ident_Proper bottom'_Proper extract_list_state_length extract_list_state_rel is_annotated_for_Proper.
+          Proof using abstract_interp_ident_Proper annotate_ident_Proper bottom'_Proper extract_list_state_length extract_list_state_rel extract_option_state_rel is_annotated_for_Proper.
             constructor; eapply wf_reflect;
               solve [ apply bottom'_Proper
                     | apply wf_annotate
@@ -610,41 +622,41 @@ Module Compilers.
 
           Lemma wf_interp_ident (annotate_with_state : bool) G {t} idc1 idc2 (Hidc : idc1 = idc2)
             : wf_value_with_lets G (@interp_ident1 annotate_with_state t idc1) (@interp_ident2 annotate_with_state t idc2).
-          Proof using abstract_interp_ident_Proper annotate_ident_Proper bottom'_Proper extract_list_state_length extract_list_state_rel is_annotated_for_Proper.
+          Proof using abstract_interp_ident_Proper annotate_ident_Proper bottom'_Proper extract_list_state_length extract_list_state_rel extract_option_state_rel is_annotated_for_Proper.
             cbv [wf_value_with_lets ident.interp_ident]; subst idc2; destruct idc1;
               first [ apply wf_interp_ident_nth_default
                     | apply wf_interp_ident_not_nth_default ].
           Qed.
 
-          Local Notation eval_with_bound1 := (@partial.ident.eval_with_bound var1 abstract_domain' annotate_ident bottom' abstract_interp_ident extract_list_state is_annotated_for).
-          Local Notation eval_with_bound2 := (@partial.ident.eval_with_bound var2 abstract_domain' annotate_ident bottom' abstract_interp_ident extract_list_state is_annotated_for).
+          Local Notation eval_with_bound1 := (@partial.ident.eval_with_bound var1 abstract_domain' annotate_ident bottom' abstract_interp_ident extract_list_state extract_option_state is_annotated_for).
+          Local Notation eval_with_bound2 := (@partial.ident.eval_with_bound var2 abstract_domain' annotate_ident bottom' abstract_interp_ident extract_list_state extract_option_state is_annotated_for).
           Lemma wf_eval_with_bound (annotate_with_state : bool) {t} G G' e1 e2 (Hwf : expr.wf G e1 e2) st1 st2 (Hst : type.and_for_each_lhs_of_arrow (@abstract_domain_R) st1 st2)
                 (HGG' : forall t v1 v2, List.In (existT _ t (v1, v2)) G -> wf_value_with_lets G' v1 v2)
             : expr.wf G' (@eval_with_bound1 annotate_with_state t e1 st1) (@eval_with_bound2 annotate_with_state t e2 st2).
-          Proof using abstract_interp_ident_Proper annotate_ident_Proper bottom'_Proper extract_list_state_length extract_list_state_rel is_annotated_for_Proper.
+          Proof using abstract_interp_ident_Proper annotate_ident_Proper bottom'_Proper extract_list_state_length extract_list_state_rel extract_option_state_rel is_annotated_for_Proper.
             eapply wf_eval_with_bound';
               solve [ eassumption
                     | eapply wf_annotate
                     | eapply wf_interp_ident ].
           Qed.
 
-          Local Notation eval1 := (@partial.ident.eval var1 abstract_domain' annotate_ident bottom' abstract_interp_ident extract_list_state is_annotated_for).
-          Local Notation eval2 := (@partial.ident.eval var2 abstract_domain' annotate_ident bottom' abstract_interp_ident extract_list_state is_annotated_for).
+          Local Notation eval1 := (@partial.ident.eval var1 abstract_domain' annotate_ident bottom' abstract_interp_ident extract_list_state extract_option_state is_annotated_for).
+          Local Notation eval2 := (@partial.ident.eval var2 abstract_domain' annotate_ident bottom' abstract_interp_ident extract_list_state extract_option_state is_annotated_for).
           Lemma wf_eval {t} G G' e1 e2 (Hwf : expr.wf G e1 e2)
                 (HGG' : forall t v1 v2, List.In (existT _ t (v1, v2)) G -> wf_value_with_lets G' v1 v2)
             : expr.wf G' (@eval1 t e1) (@eval2 t e2).
-          Proof using abstract_interp_ident_Proper annotate_ident_Proper bottom'_Proper extract_list_state_length extract_list_state_rel is_annotated_for_Proper.
+          Proof using abstract_interp_ident_Proper annotate_ident_Proper bottom'_Proper extract_list_state_length extract_list_state_rel extract_option_state_rel is_annotated_for_Proper.
             eapply wf_eval';
               solve [ eassumption
                     | eapply wf_annotate
                     | eapply wf_interp_ident ].
           Qed.
 
-          Local Notation eta_expand_with_bound1 := (@partial.ident.eta_expand_with_bound var1 abstract_domain' annotate_ident bottom' abstract_interp_ident extract_list_state is_annotated_for).
-          Local Notation eta_expand_with_bound2 := (@partial.ident.eta_expand_with_bound var2 abstract_domain' annotate_ident bottom' abstract_interp_ident extract_list_state is_annotated_for).
+          Local Notation eta_expand_with_bound1 := (@partial.ident.eta_expand_with_bound var1 abstract_domain' annotate_ident bottom' abstract_interp_ident extract_list_state extract_option_state is_annotated_for).
+          Local Notation eta_expand_with_bound2 := (@partial.ident.eta_expand_with_bound var2 abstract_domain' annotate_ident bottom' abstract_interp_ident extract_list_state extract_option_state is_annotated_for).
           Lemma wf_eta_expand_with_bound {t} G e1 e2 (Hwf : expr.wf G e1 e2) st1 st2 (Hst : type.and_for_each_lhs_of_arrow (@abstract_domain_R) st1 st2)
             : expr.wf G (@eta_expand_with_bound1 t e1 st1) (@eta_expand_with_bound2 t e2 st2).
-          Proof using abstract_interp_ident_Proper annotate_ident_Proper bottom'_Proper extract_list_state_length extract_list_state_rel is_annotated_for_Proper.
+          Proof using abstract_interp_ident_Proper annotate_ident_Proper bottom'_Proper extract_list_state_length extract_list_state_rel extract_option_state_rel is_annotated_for_Proper.
             eapply wf_eta_expand_with_bound';
               solve [ eassumption
                     | eapply wf_annotate
@@ -682,6 +694,8 @@ Module Compilers.
                        | progress destruct_head'_prod
                        | progress destruct_head'_bool
                        | progress destruct_head' option
+                       | progress inversion_option
+                       | discriminate
                        | solve [ eauto ]
                        | apply NatUtil.nat_rect_Proper_nondep
                        | apply ListUtil.list_rect_Proper
@@ -691,8 +705,15 @@ Module Compilers.
                        | apply ListUtil.update_nth_Proper
                        | apply (@nat_rect_Proper_nondep_gen (_ -> _) (eq ==> eq)%signature)
                        | cbn; apply (f_equal (@Some _))
+                       | progress cbn [ZRange.ident.option.interp]
+                       | progress cbv [zrange_rect]
+                       | apply (f_equal2 pair)
+                       | break_innermost_match_step
                        | match goal with
                          | [ H : _ |- _ ] => erewrite H by (eauto; (eassumption || reflexivity))
+                         | [ H : forall x y, x = y -> _ |- _ ] => specialize (fun x => H x x eq_refl)
+                         | [ H : forall x, ?f x = ?g x, H1 : ?f ?y = _, H2 : ?g ?y = _ |- _ ]
+                           => specialize (H y); rewrite H1, H2 in H
                          end ].
       Qed.
 
@@ -719,6 +740,12 @@ Module Compilers.
         destruct_head'_ex; destruct_head'_and; inversion_prod; subst; reflexivity.
       Qed.
 
+      Lemma extract_option_state_rel
+        : forall t v1 v2, abstract_domain'_R _ v1 v2 -> option_eq (option_eq (abstract_domain'_R _)) (extract_option_state t v1) (extract_option_state t v2).
+      Proof.
+        cbv [extract_option_state option_eq]; intros; subst; break_match; reflexivity.
+      Qed.
+
       Section with_var2.
         Context {var1 var2 : type -> Type}.
         Local Notation wf_value_with_lets := (@wf_value_with_lets base.type ident abstract_domain' (fun t => abstract_domain'_R t) var1 var2).
@@ -731,7 +758,8 @@ Module Compilers.
             solve [ eassumption
                   | exact _
                   | apply extract_list_state_length
-                  | apply extract_list_state_rel ].
+                  | apply extract_list_state_rel
+                  | apply extract_option_state_rel ].
         Qed.
 
         Lemma wf_eval_with_bound {relax_zrange t} G G' e1 e2 (Hwf : expr.wf G e1 e2) st1 st2 (Hst : type.and_for_each_lhs_of_arrow (@abstract_domain_R) st1 st2)
@@ -742,7 +770,8 @@ Module Compilers.
             solve [ eassumption
                   | exact _
                   | apply extract_list_state_length
-                  | apply extract_list_state_rel ].
+                  | apply extract_list_state_rel
+                  | apply extract_option_state_rel ].
         Qed.
 
 
@@ -753,7 +782,8 @@ Module Compilers.
             solve [ eassumption
                   | exact _
                   | apply extract_list_state_length
-                  | apply extract_list_state_rel ].
+                  | apply extract_list_state_rel
+                  | apply extract_option_state_rel ].
         Qed.
       End with_var2.
 
